compiler/inference/proofs/inferSoundScript.sml
@@ -736,7 +736,7 @@ Theorem db_subst_infer_subst_swap2:
 Proof
 ho_match_mp_tac infer_t_induction >>
 rw [convert_t_def, deBruijn_subst_def, EL_MAP, t_walkstar_eqn1,
-    infer_deBruijn_subst_def, MAP_MAP_o, combinTheory.o_DEF, check_t_def,
+    infer_deBruijn_subst_alt, MAP_MAP_o, combinTheory.o_DEF, check_t_def,
     LENGTH_COUNT_LIST]
 QED
 
